rhombus-hol/info.rkt
@@ -1,0 +1,12 @@
+#lang info
+
+(define collection 'multi)
+(define deps '("base" "rhombus-hol-prover" "rhombus-hol-kernel"
+               "rhombus-hol-quickcheck" "rhombus-hol-stdlib"))
+(define implies '("rhombus-hol-prover" "rhombus-hol-kernel"
+                  "rhombus-hol-quickcheck"))
+(define build-deps '("rhombus" "rhombus-scribble-lib"))
+(define pkg-desc "Rhombus/HOL: a theorem prover embedded in Rhombus")
+(define license '0BSD)
+(define version "0.1")
+(define language-families '("Rhombus"))
